Working on StackAware

backend/Cminor.v
@@ -243,6 +243,10 @@ Inductive state: Type :=
              (m: mem),                  (**r memory state *)
       state.
 
+Section ORACLE.
+
+Variable fn_stack_requirements : ident -> Z.
+
 Section RELSEM.
 
 Variable ge: genv.
@@ -443,6 +447,7 @@ Inductive step: state -> trace -> state -> Prop :=
       is_call_cont k ->
       Mem.free m sp 0 f.(fn_stackspace) = Some m' ->
       Mem.return_frame m' = Some m'' ->
+      Mem.astack (Mem.support m'') <> nil ->
       step (State f Sskip k (Vptr sp Ptrofs.zero) e m)
         E0 (Returnstate Vundef k m'')
 
@@ -465,7 +470,7 @@ Inductive step: state -> trace -> state -> Prop :=
       Genv.find_funct ge vf = Some fd ->
       funsig fd = sig ->
       step (State f (Scall optid sig a bl) k sp e m)
-        E0 (Callstate fd vargs (Kcall optid f sp e k) m id)
+        E0 (Callstate fd vargs (Kcall optid f sp e k) (Mem.push_stage m) id)
 
   | step_tailcall: forall f sig a bl k sp e m vf vargs fd m' m'' id,
       vf = Vptr (Global id) Ptrofs.zero ->
@@ -475,14 +480,16 @@ Inductive step: state -> trace -> state -> Prop :=
       funsig fd = sig ->
       Mem.free m sp 0 f.(fn_stackspace) = Some m' ->
       Mem.return_frame m' = Some m'' ->
+      Mem.astack (Mem.support m'') <> nil ->
       step (State f (Stailcall sig a bl) k (Vptr sp Ptrofs.zero) e m)
         E0 (Callstate fd vargs (call_cont k) m'' id)
 
-  | step_builtin: forall f optid ef bl k sp e m vargs t vres m',
+  | step_builtin: forall f optid ef bl k sp e m vargs t vres m' m'',
       eval_exprlist sp e m bl vargs ->
-      external_call ef ge vargs m t vres m' ->
+      external_call ef ge vargs (Mem.push_stage m) t vres m' ->
+      Mem.pop_stage m' = Some m'' ->
       step (State f (Sbuiltin optid ef bl) k sp e m)
-         t (State f Sskip k sp (set_optvar optid vres e) m')
+         t (State f Sskip k sp (set_optvar optid vres e) m'')
 
   | step_seq: forall f s1 s2 k sp e m,
       step (State f (Sseq s1 s2) k sp e m)
@@ -521,12 +528,14 @@ Inductive step: state -> trace -> state -> Prop :=
   | step_return_0: forall f k sp e m m' m'',
       Mem.free m sp 0 f.(fn_stackspace) = Some m' ->
       Mem.return_frame m' = Some m'' ->
+      Mem.astack (Mem.support m'') <> nil ->
       step (State f (Sreturn None) k (Vptr sp Ptrofs.zero) e m)
         E0 (Returnstate Vundef (call_cont k) m'')
   | step_return_1: forall f a k sp e m v m' m'',
       eval_expr (Vptr sp Ptrofs.zero) e m a v ->
       Mem.free m sp 0 f.(fn_stackspace) = Some m' ->
       Mem.return_frame m' = Some m'' ->
+      Mem.astack (Mem.support m'') <> nil ->
       step (State f (Sreturn (Some a)) k (Vptr sp Ptrofs.zero) e m)
         E0 (Returnstate v (call_cont k) m'')
 
@@ -539,20 +548,22 @@ Inductive step: state -> trace -> state -> Prop :=
       step (State f (Sgoto lbl) k sp e m)
         E0 (State f s' k' sp e m)
 
-  | step_internal_function: forall f vargs k m m' m'' sp e path id,
+  | step_internal_function: forall f vargs k m m' m'' m''' sp e path id,
       Mem.alloc_frame m id = (m', path) ->
       Mem.alloc m' 0 f.(fn_stackspace) = (m'', sp) ->
+      Mem.record_frame m'' (mk_frame (fn_stack_requirements id)) = Some m''' ->
       set_locals f.(fn_vars) (set_params vargs f.(fn_params)) = e ->
       step (Callstate (Internal f) vargs k m id)
-        E0 (State f f.(fn_body) k (Vptr sp Ptrofs.zero) e m'')
+        E0 (State f f.(fn_body) k (Vptr sp Ptrofs.zero) e m''')
   | step_external_function: forall ef vargs k m t vres m' id,
       external_call ef ge vargs m t vres m' ->
       step (Callstate (External ef) vargs k m id)
          t (Returnstate vres k m')
 
-  | step_return: forall v optid f sp e k m,
+  | step_return: forall v optid f sp e k m m',
+      Mem.pop_stage m = Some m' ->
       step (Returnstate v (Kcall optid f sp e k) m)
-        E0 (State f Sskip k sp (set_optvar optid v e) m).
+        E0 (State f Sskip k sp (set_optvar optid v e) m').
 
 End RELSEM.
 
@@ -568,7 +579,7 @@ Inductive initial_state (p: program): state -> Prop :=
       Genv.find_symbol ge p.(prog_main) = Some b ->
       Genv.find_funct_ptr ge b = Some f ->
       funsig f = signature_main ->
-      initial_state p (Callstate f nil Kstop m0 p.(prog_main)).
+      initial_state p (Callstate f nil Kstop (Mem.push_stage m0) p.(prog_main)).
 
 (** A final state is a [Returnstate] with an empty continuation. *)
 
@@ -592,12 +603,23 @@ Proof.
     intros. subst. inv H0. exists s1; auto.
   inversion H; subst; auto.
   exploit external_call_receptive; eauto. intros [vres2 [m2 EC2]].
-  exists (State f Sskip k sp (set_optvar optid vres2 e) m2). econstructor; eauto.
+  assert ({m3:mem | Mem.pop_stage m2 = Some m3}).
+    apply Mem.nonempty_pop_stage.
+    admit.
+    (*
+    eapply external_call_mem_stackeq in EC2.
+    eapply external_call_mem_stackeq in H3.
+    unfold Mem.stackeq in *.
+    rewrite <- EC2. rewrite H3. apply Mem.pop_stage_nonempty in H4.
+    auto.
+    *)
+  destruct X as [m3 POP_STAGE].
+  exists (State f Sskip k sp (set_optvar optid vres2 e) m3). econstructor; eauto.
   exploit external_call_receptive; eauto. intros [vres2 [m2 EC2]].
   exists (Returnstate vres2 k m2). econstructor; eauto.
 (* trace length *)
   red; intros; inv H; simpl; try lia; eapply external_call_trace_length; eauto.
-Qed.
+Admitted.
 
 (** This semantics is determinate. *)
 
@@ -644,7 +666,7 @@ Proof.
   intros. constructor; set (ge := Genv.globalenv p); simpl; intros.
 - (* determ *)
   inv H; inv H0; Determ.
-  + subst vargs0. exploit external_call_determ. eexact H2. eexact H13.
+  + subst vargs0. exploit external_call_determ. eexact H2. eexact H14.
     intros (A & B). split; intros; auto.
     apply B in H; destruct H; congruence.
   + subst v0. assert (b0 = b) by (inv H2; inv H13; auto). subst b0; auto.
@@ -663,6 +685,7 @@ Proof.
   inv H; inv H0; auto.
 Qed.
 
+End ORACLE.
 (** * Alternate operational semantics (big-step)
 
 (** We now define another semantics for Cminor without [goto] that follows
