common/Memory.v
@@ -624,18 +624,91 @@ Qed.
 
 End STREE.
 
+Section STACKADT.
+
+Record frame : Type :=
+  {
+    frame_size : Z;
+    frame_size_pos:
+      (0 <= frame_size)%Z;
+  }.
+
+Definition mk_frame (sz:Z) :=
+  {|
+   frame_size := Z.max 0 sz;
+   frame_size_pos := Z.le_max_l _ _
+  |}.
+
+Definition stage := list frame.
+
+Fixpoint size_of_all_frames (t:stage) : Z :=
+  match t with
+    |nil => 0
+    |hd :: tl => (frame_size hd) + size_of_all_frames tl
+  end.
+(*
+Definition size_of_head_frame (t:stage) : Z :=
+  match t with
+    |nil => 0
+    |hd::tl => (frame_size hd)
+  end.
+*)
+Definition stackadt := list stage.
+
+Fixpoint stack_size (s:stackadt): Z :=
+  match s with
+    |nil => 0
+    |hd::tl => size_of_all_frames hd + stack_size tl
+  end.
+
+Lemma stack_size_app : forall s1 s2,
+    stack_size (s1++s2) = stack_size s1 + stack_size s2.
+Proof.
+  intros. induction s1. auto. simpl. lia.
+Qed.
+
+Lemma size_of_all_frames_pos:
+  forall t,
+    (0 <= size_of_all_frames t)%Z.
+Proof.
+  intros. induction t.
+  simpl. lia.
+  simpl. generalize (frame_size_pos a). intro.
+  lia.
+Qed.
+
+Lemma stack_size_pos:
+  forall s,
+    (0 <= stack_size s)%Z.
+Proof.
+  induction s; simpl; intros; eauto. lia.
+  generalize (size_of_all_frames_pos a); lia.
+Qed.
+
+Lemma stack_size_tl:
+  forall l,
+    (stack_size (tl l) <= stack_size l)%Z.
+Proof.
+  induction l; simpl; intros. lia.
+  generalize (size_of_all_frames_pos a); lia.
+Qed.
+
+Definition max_stacksize : Z := 4096.
+End STACKADT.
+
 (* Declare Module Sup: SUP. *)
 
 Module Sup <: SUP.
 
 Record sup' : Type := mksup {
   stack : stree;
+  astack : stackadt;
   global : list ident;
 }.
 
 Definition sup := sup'.
 
-Definition sup_empty : sup := mksup empty_stree nil.
+Definition sup_empty : sup := mksup empty_stree nil nil.
 
 Definition sup_cpath (s:sup) := cpath (stack s).
 
@@ -678,7 +751,7 @@ Qed.
 
 Definition sup_incr (s:sup):sup :=
   let (pp,t') := next_block_stree (stack s) in
-  mksup t' (global s).
+  mksup t' (astack s) (global s).
 
 Definition sup_include(s1 s2:sup) := forall b, sup_In b s1 -> sup_In b s2.
 
@@ -723,7 +796,7 @@ Qed.
 (* sup_incr_frame *)
 Definition sup_incr_frame (s:sup)(id:ident):sup :=
   let (t',p) := next_stree (stack s) id in
-  mksup t' (global s).
+  mksup t' (astack s)(global s).
 
 Theorem sup_incr_frame_in : forall s b id,
     sup_In b s <-> sup_In b (sup_incr_frame s id).
@@ -741,7 +814,7 @@ Qed.
 (* sup_return_frame *)
 Definition sup_return_frame (s:sup) : option sup :=
   match return_stree (stack s) with
-    |Some (t',p) => Some (mksup t' (global s))
+    |Some (t',p) => Some (mksup t' (astack s)(global s))
     |None => None
   end.
 
@@ -789,7 +862,7 @@ Qed.
 
 (* sup_incr_glob *)
 Definition sup_incr_glob (i:ident) (s:sup) : sup :=
- mksup (stack s) (i::(global s)).
+ mksup (stack s) (astack s)(i::(global s)).
 
 Theorem sup_incr_glob_in :  forall i s b,
     sup_In b (sup_incr_glob i s) <-> b = (Global i) \/ sup_In b s.
@@ -811,6 +884,47 @@ Proof. intros. intro. intro. apply sup_incr_glob_in. right. auto. Qed.
 
 Definition sup_incr_block := sup_incr.
 
+(* about stackadt *)
+
+Definition sup_push_stage (s:sup) := mksup (stack s) (nil::(astack s)) (global s).
+
+Definition sup_record_frame (f:frame)(s:sup) :=
+  match (astack s) with
+    |nil => None
+    |hd::tl => Some(mksup (stack s) ((f::hd)::tl) (global s))
+  end.
+
+Definition sup_pop_stage (s:sup) :=
+  match (astack s) with
+  |nil => None
+  |hd::tl => Some(mksup (stack s) (tl)(global s))
+  end.
+
+(*
+Theorem sup_push_stage_stack : forall s, stack s = stack (sup_push_stage s).
+Proof.
+  intros. unfold sup_push_stage. reflexivity. Qed.
+
+Theorem sup_push_stage_global : forall s, global s = global (sup_push_stage s).
+Proof.
+  intros. unfold sup_push_stage. reflexivity. Qed.
+
+Theorem sup_record_frame_stack :forall sz s s', sup_record_frame sz s = Some s' -> stack s = stack s'.
+Proof.
+  intros. unfold sup_record_frame in H. destruct (astack s). discriminate. simpl in H. inv H.  reflexivity.
+Qed.
+
+Theorem sup_record_frame_global :forall sz s s', sup_record_frame sz s = Some s' -> stack s = stack s'.
+Proof.
+  intros. unfold sup_record_frame in H. destruct (astack s). discriminate. simpl in H. inv H.  reflexivity.
+Qed.
+
+Theorem sup_pop_stage_supp : forall s s', sup_pop_stage s = Some s' -> supp s = supp s'.
+Proof.
+  intros. unfold sup_pop_stage in H.  destruct (stack s); auto. discriminate.
+  inv H. reflexivity.
+Qed.
+*)
 End Sup.
 
 Module Mem <: MEM.
@@ -1274,6 +1388,50 @@ Qed.
 Next Obligation.
   rewrite NMap.gsspec. destruct (NMap.elt_eq b (nextblock m)). auto. apply contents_default.
 Qed.
+
+Program Definition push_stage (m:mem):=
+  (mkmem m.(mem_contents)
+         m.(mem_access)
+         (sup_push_stage m.(support))
+         m.(access_max)
+         m.(nextblock_noaccess)
+         m.(contents_default)
+  ).
+
+Program Definition pop_stage (m:mem) :=
+  match astack (support m) with
+    |hd::tl =>
+       Some (mkmem m.(mem_contents)
+         m.(mem_access)
+         (mksup (stack (support m)) tl (global (support m)))
+         m.(access_max)
+         m.(nextblock_noaccess)
+         m.(contents_default)
+  )
+    |nil => None
+  end.
+
+Lemma pop_push_stage : forall m, pop_stage (push_stage m) = Some m.
+Proof.
+  intro. unfold push_stage.
+  unfold pop_stage. simpl. apply f_equal.
+  destruct m. simpl. apply mkmem_ext; auto.
+  destruct support0. reflexivity.
+Qed.
+
+Program Definition record_frame (m:mem)(fr:frame) :=
+  if (zle (frame_size fr + (stack_size (astack (support m)))) max_stacksize) then
+  match astack (support m) with
+    |hd::tl =>
+       Some (mkmem m.(mem_contents)
+         m.(mem_access)
+         (mksup (stack (support m)) ((fr::hd)::tl) (global (support m)))
+         m.(access_max)
+         m.(nextblock_noaccess)
+         m.(contents_default)
+  )
+    |nil => None
+  end else None.
 
 (** Freeing a block between the given bounds.
   Return the updated memory state where the given range of the given block
@@ -2627,6 +2785,13 @@ Proof.
   reflexivity.
 Qed.
 
+Lemma astack_alloc_frame:
+  astack (support m1) = astack (support m2).
+Proof.
+  rewrite support_alloc_frame. unfold sup_incr_frame.
+  destr.
+Qed.
+
 Lemma path_alloc_frame:
     path = sup_npath (support m1) id.
 Proof.
@@ -2762,6 +2927,14 @@ Proof.
   generalize support_return_frame.
   intro. unfold sup_return_frame in H.
   destr_in H. destruct p. inv H. eauto.
+Qed.
+
+Lemma astack_return_frame:
+  astack (support m1) = astack (support m2).
+Proof.
+  generalize support_return_frame.
+  intro. unfold sup_return_frame in H.
+  repeat destr_in H. inv H1. simpl. congruence.
 Qed.
 
 Lemma sup_include_return_frame :
@@ -3059,7 +3232,7 @@ Local Hint Resolve valid_access_alloc_other valid_access_alloc_same: mem.
 
 Section ALLOCF_ALLOC.
 Local Set Elimination Schemes.
-Local Set Analysis Schemes.
+
 Inductive alloc_vars_left : mem -> list block -> mem -> Prop :=
   |avl_nil : forall m, alloc_vars_left m nil m
   |avl_cons : forall m m1 m2 blocks b sz,
@@ -3281,6 +3454,359 @@ Proof.
 Qed.
 
 End ALLOCGLOB.
+
+Section PUSH_STAGE.
+
+Variable m1: mem.
+Variable m2: mem.
+Hypothesis PUSH_STAGE: push_stage m1 = m2.
+
+Lemma support_push_stage :
+    support m2 = sup_push_stage (support m1).
+Proof.
+  intros. unfold push_stage in PUSH_STAGE. rewrite <- PUSH_STAGE.
+  reflexivity.
+Qed.
+
+Theorem nextblock_push_stage:
+  nextblock m2 = nextblock m1.
+Proof.
+  unfold nextblock. rewrite support_push_stage. unfold fresh_block.
+  reflexivity.
+Qed.
+
+Theorem valid_block_push_stage_1:
+  forall b, valid_block m1 b -> valid_block m2 b.
+Proof.
+  unfold valid_block. rewrite support_push_stage. auto.
+Qed.
+
+Theorem valid_block_push_stage_2:
+  forall b, valid_block m2 b -> valid_block m1 b.
+Proof.
+  unfold valid_block. rewrite support_push_stage. auto.
+Qed.
+
+Local Hint Resolve valid_block_push_stage_1 valid_block_push_stage_2: mem.
+
+Theorem perm_push_stage:
+  forall b ofs k p,
+  perm m1 b ofs k p <->
+  perm m2 b ofs k p.
+Proof.
+  inv PUSH_STAGE. unfold perm. reflexivity.
+Qed.
+
+Theorem valid_access_push_stage:
+  forall chunk b ofs p,
+  valid_access m1 chunk b ofs p <->
+  valid_access m2 chunk b ofs p.
+Proof.
+  inv PUSH_STAGE. reflexivity.
+Qed.
+
+Theorem load_push_stage:
+  forall chunk b ofs,
+  load chunk m2 b ofs = load chunk m1 b ofs.
+Proof.
+  intros. unfold load.
+  destruct (valid_access_dec m2 chunk b ofs Readable).
+  rewrite pred_dec_true. rewrite <- PUSH_STAGE. reflexivity.
+  eapply valid_access_push_stage; eauto.
+  rewrite pred_dec_false; auto.
+  red; intro; elim n. eapply valid_access_push_stage; eauto.
+Qed.
+
+Theorem load_push_stage_2:
+  forall chunk b ofs v,
+  load chunk m2 b ofs = Some v -> load chunk m1 b ofs = Some v.
+Proof.
+  intros. unfold load. rewrite pred_dec_true.
+  rewrite (load_result _ _ _ _ _ H). rewrite <- PUSH_STAGE. reflexivity.
+  apply valid_access_push_stage. eauto with mem.
+Qed.
+
+Theorem loadbytes_push_stage:
+  forall b ofs n,
+  loadbytes m2 b ofs n = loadbytes m1 b ofs n.
+Proof.
+  intros. unfold loadbytes.
+  destruct (range_perm_dec m2 b ofs (ofs + n) Cur Readable).
+  rewrite pred_dec_true.
+  rewrite <- PUSH_STAGE. reflexivity.
+  red; intros. eapply perm_push_stage; eauto.
+  rewrite pred_dec_false; auto.
+  red; intros. elim n0; red; intros.
+  eapply perm_push_stage; eauto.
+Qed.
+
+End PUSH_STAGE.
+
+Lemma nonempty_pop_stage : forall m1,
+   astack (support m1) <> nil -> {m2:mem|pop_stage m1 = Some m2}.
+Proof.
+  intros; unfold pop_stage. destruct (astack (support m1)). congruence.
+  econstructor; eauto.
+Qed.
+
+Section POP_STAGE.
+
+Variable m1: mem.
+Variable m2: mem.
+Hypothesis POP_STAGE: pop_stage m1 = Some m2.
+
+Lemma pop_stage_nonempty :
+   astack (support m1) <> nil.
+Proof.
+  intros. unfold pop_stage in POP_STAGE. destruct (astack(support m1)); auto.
+  discriminate. congruence.
+Qed.
+
+Lemma support_pop_stage :
+    sup_pop_stage (support m1) = Some (support m2).
+Proof.
+  intros.  unfold pop_stage in POP_STAGE. destruct (astack(support m1)) eqn:H0; auto.
+  discriminate. inv POP_STAGE. unfold sup_pop_stage. simpl. rewrite H0. auto.
+Qed.
+
+Lemma astack_pop_stage:
+      exists hd,
+        astack(support m1) = hd :: (astack(support m2)).
+Proof.
+  intros.
+  unfold pop_stage in POP_STAGE.
+  destruct (astack (support m1)).
+  discriminate.
+  inv POP_STAGE. simpl.
+  exists s. auto.
+Qed.
+
+Lemma stack_pop_stage :
+  stack (support m1) = stack (support m2).
+Proof.
+  unfold pop_stage in POP_STAGE. destruct (astack (support m1)).
+  discriminate. inv POP_STAGE. auto.
+Qed.
+
+Lemma global_pop_stage :
+  global (support m1) = global (support m2).
+Proof.
+  unfold pop_stage in POP_STAGE. destruct (astack (support m1)).
+  discriminate. inv POP_STAGE. auto.
+Qed.
+
+Lemma sup_include_pop_stage :
+  sup_include (support m1) (support m2).
+Proof.
+  unfold sup_include, sup_In.  rewrite stack_pop_stage.
+  rewrite global_pop_stage. auto.
+Qed.
+
+Theorem nextblock_pop_stage:
+  nextblock m2 = nextblock m1.
+Proof.
+  unfold nextblock. unfold fresh_block.
+  rewrite stack_pop_stage. reflexivity.
+Qed.
+
+Theorem valid_block_pop_stage_1:
+  forall b, valid_block m1 b -> valid_block m2 b.
+Proof.
+  unfold valid_block, sup_In. rewrite stack_pop_stage.
+  rewrite global_pop_stage. auto.
+Qed.
+
+Theorem valid_block_pop_stage_2:
+  forall b, valid_block m2 b -> valid_block m1 b.
+Proof.
+  unfold valid_block, sup_In. rewrite stack_pop_stage.
+  rewrite global_pop_stage. auto.
+Qed.
+
+Local Hint Resolve valid_block_pop_stage_1 valid_block_pop_stage_2: mem.
+
+Theorem perm_pop_stage:
+  forall b ofs k p,
+  perm m1 b ofs k p <->
+  perm m2 b ofs k p.
+Proof.
+  intros. unfold pop_stage in POP_STAGE. destruct (astack(support m1)); auto.
+  discriminate. inv POP_STAGE. auto. reflexivity.
+Qed.
+
+
+Theorem valid_access_pop_stage:
+  forall chunk b ofs p,
+  valid_access m1 chunk b ofs p <->
+  valid_access m2 chunk b ofs p.
+Proof.
+  split;(
+  intros; inv H; constructor; auto with mem;
+  red; intros; eapply perm_pop_stage; eauto ).
+Qed.
+
+Theorem load_pop_stage:
+  forall chunk b ofs,
+  load chunk m2 b ofs = load chunk m1 b ofs.
+Proof.
+  intros. unfold pop_stage in POP_STAGE. destruct (astack(support m1)); auto. discriminate. inv POP_STAGE. simpl. reflexivity.
+Qed.
+
+Theorem loadbytes_pop_stage:
+  forall b ofs n,
+  loadbytes m2 b ofs n = loadbytes m1 b ofs n.
+Proof.
+  intros. unfold pop_stage in POP_STAGE. destruct (astack(support m1)); auto. discriminate. inv POP_STAGE. simpl. reflexivity.
+Qed.
+
+End POP_STAGE.
+
+Local Hint Resolve valid_block_pop_stage_1 valid_block_pop_stage_2
+             perm_pop_stage
+             valid_access_pop_stage: mem.
+
+Lemma request_record_frame : forall m1 fr,
+   astack (support m1) <> nil  ->
+    frame_size fr  + stack_size (astack(support m1)) <= max_stacksize
+   -> {m2:mem| record_frame m1 fr = Some m2}.
+Proof.
+  intros; unfold record_frame. rewrite zle_true.
+  destruct (astack (support m1)); simpl.
+  congruence. simpl in *. eauto. lia.
+Qed.
+
+Section RECORD_FRAME.
+
+Variable m1: mem.
+Variable m2: mem.
+Variable fr: frame.
+
+Hypothesis RECORD_FRAME: record_frame m1 fr = Some m2.
+
+Lemma record_frame_size :
+    (stack_size (astack(support m2))) <= max_stacksize.
+Proof.
+  intros. unfold record_frame in RECORD_FRAME.   repeat destr_in RECORD_FRAME.
+  simpl in *. lia.
+Qed.
+
+Lemma record_frame_size1:
+  (frame_size fr + stack_size (astack (support m1))) <= max_stacksize.
+Proof.
+  intros. unfold record_frame in RECORD_FRAME.   repeat destr_in RECORD_FRAME.
+Qed.
+
+Lemma record_frame_nonempty :
+   astack (support m1) <> nil.
+Proof.
+  intros. unfold record_frame in RECORD_FRAME. repeat destr_in RECORD_FRAME.
+Qed.
+
+Lemma support_record_frame :
+    sup_record_frame fr (support m1) = Some (support m2).
+Proof.
+  intros. unfold record_frame in RECORD_FRAME.
+  repeat destr_in RECORD_FRAME. unfold sup_record_frame. rewrite Heqs.
+  reflexivity.
+Qed.
+
+Lemma astack_record_frame : exists hd tl,
+  astack (support m1) = hd::tl /\
+  astack (support m2) = (fr::hd)::tl.
+Proof.
+  intros. generalize support_record_frame. unfold sup_record_frame. intro.
+  generalize record_frame_nonempty.
+  destruct (astack (support m1)). intro.
+  discriminate. inv RECORD_FRAME. intro. inv H.
+  exists s. exists s0. auto.
+Qed.
+
+Lemma stack_record_frame :
+  stack (support m1) = stack (support m2).
+Proof.
+  intros. unfold record_frame in RECORD_FRAME.
+  repeat destr_in RECORD_FRAME. reflexivity.
+Qed.
+
+Lemma global_record_frame :
+  global (support m1) = global (support m2).
+Proof.
+  intros. unfold record_frame in RECORD_FRAME.
+  repeat destr_in RECORD_FRAME. reflexivity.
+Qed.
+
+Lemma sup_include_record_frame :
+  sup_include (support m1) (support m2).
+Proof.
+  unfold sup_include. unfold sup_In.
+  rewrite stack_record_frame. rewrite global_record_frame. auto.
+Qed.
+
+Theorem nextblock_record_frame:
+  nextblock m2 = nextblock m1.
+Proof.
+  unfold nextblock. unfold fresh_block.
+  rewrite stack_record_frame. auto.
+Qed.
+
+Theorem valid_block_record_frame_1:
+  forall b, valid_block m1 b -> valid_block m2 b.
+Proof.
+  unfold valid_block. unfold sup_In.
+  rewrite stack_record_frame. rewrite global_record_frame. auto.
+Qed.
+
+Theorem valid_block_record_frame_2:
+  forall b, valid_block m2 b -> valid_block m1 b.
+Proof.
+  unfold valid_block. unfold sup_In.
+  rewrite stack_record_frame. rewrite global_record_frame. auto.
+Qed.
+
+Local Hint Resolve valid_block_record_frame_1 valid_block_record_frame_2: mem.
+
+Theorem perm_record_frame:
+  forall b ofs k p,
+  perm m1 b ofs k p <->
+  perm m2 b ofs k p.
+Proof.
+  intros. unfold record_frame in RECORD_FRAME. repeat destr_in RECORD_FRAME.
+  unfold perm. reflexivity.
+Qed.
+
+Theorem valid_access_record_frame:
+  forall chunk b ofs p,
+  valid_access m1 chunk b ofs p <->
+  valid_access m2 chunk b ofs p.
+Proof.
+  split.
+  intros. inv H. constructor; auto with mem.
+  red; intros. eapply perm_record_frame; eauto.
+  intros. inv H. constructor; auto with mem.
+  red; intros. eapply perm_record_frame; eauto.
+Qed.
+
+Theorem load_record_frame:
+  forall chunk b ofs,
+  load chunk m2 b ofs = load chunk m1 b ofs.
+Proof.
+  intros. unfold record_frame in RECORD_FRAME.
+  repeat destr_in RECORD_FRAME. auto.
+Qed.
+
+Theorem loadbytes_record_frame:
+  forall b ofs n,
+  loadbytes m2 b ofs n = loadbytes m1 b ofs n.
+Proof.
+  intros. unfold record_frame in RECORD_FRAME.
+  repeat destr_in RECORD_FRAME. auto.
+Qed.
+
+End RECORD_FRAME.
+
+Local Hint Resolve valid_block_record_frame_1 valid_block_record_frame_2
+             perm_record_frame
+             valid_access_record_frame: mem.
 
 (** ** Properties related to [free]. *)
 
@@ -4200,6 +4726,64 @@ Proof.
   intros. rewrite FREE; simpl. eauto.
 Qed.
 
+Lemma push_stage_left_inj:
+  forall f m1 m2 m1',
+  mem_inj f m1 m2 ->
+  push_stage m1 = m1' ->
+  mem_inj f m1' m2.
+Proof.
+  intros. inversion H. inv H0. constructor; auto.
+Qed.
+
+Lemma push_stage_right_inj:
+  forall f m1 m2 m2',
+  mem_inj f m1 m2 ->
+  push_stage m2 = m2' ->
+  mem_inj f m1 m2'.
+Proof.
+  intros. inversion H. inv H0. constructor; auto.
+Qed.
+
+Lemma pop_stage_left_inj:
+  forall f m1 m2 m1',
+  mem_inj f m1 m2 ->
+  pop_stage m1 = Some m1' ->
+  mem_inj f m1' m2.
+Proof.
+  intros. unfold pop_stage in H0. destr_in H0.
+  inversion H. inv H0. constructor; auto.
+Qed.
+
+Lemma pop_stage_right_inj:
+  forall f m1 m2 m2',
+  mem_inj f m1 m2 ->
+  pop_stage m2 = Some m2' ->
+  mem_inj f m1 m2'.
+Proof.
+  intros. unfold pop_stage in H0. destr_in H0.
+  inversion H. inv H0. constructor; auto.
+Qed.
+
+Lemma record_frame_left_inj:
+  forall f fr m1 m2 m1',
+  mem_inj f m1 m2 ->
+  record_frame m1 fr = Some m1' ->
+  mem_inj f m1' m2.
+Proof.
+  intros. unfold record_frame in H0. repeat destr_in H0.
+  inversion H. constructor; auto.
+Qed.
+
+Lemma record_frame_right_inj:
+  forall f fr m1 m2 m2',
+  mem_inj f m1 m2 ->
+  record_frame m2 fr = Some m2' ->
+  mem_inj f m1 m2'.
+Proof.
+  intros. unfold record_frame in H0. repeat destr_in H0.
+  inversion H. constructor; auto.
+Qed.
+
 (** Preservation of [drop_perm] operations. *)
 
 Lemma drop_unmapped_inj:
@@ -4498,6 +5082,136 @@ Proof.
   - eauto.
 Qed.
 
+Theorem push_stage_extends:
+  forall m1 m2,
+  extends m1 m2 ->
+  extends (push_stage m1) (push_stage m2).
+Proof.
+  intros. inv H.
+  constructor; unfold push_stage;simpl.
+  - rewrite mext_sup0. reflexivity.
+  - inv mext_inj0. constructor; auto.
+  - auto.
+Qed.
+
+Theorem pop_stage_extends:
+  forall m1 m1' m2,
+  extends m1 m2 ->
+  pop_stage m1 = Some m1' ->
+  exists m2', pop_stage m2 = Some m2' /\
+         extends m1' m2'.
+Proof.
+  intros. inv H.
+  apply pop_stage_nonempty in H0 as H1.
+  rewrite mext_sup0 in H1.
+  apply nonempty_pop_stage in H1.
+  destruct H1 as [m2' POP]. exists m2'.
+  split. auto.
+  constructor; eauto.
+  - apply support_pop_stage in H0.
+    apply support_pop_stage in POP.
+    congruence.
+  - eapply pop_stage_right_inj with (m1 := m1'); eauto.
+    eapply pop_stage_left_inj; eauto.
+  - intros. exploit mext_perm_inv0.
+    eapply perm_pop_stage in POP; eauto. apply POP in H. apply H.
+    intros [A|A].
+    eapply perm_pop_stage in H0; eauto. left. apply H0. auto.
+    right; intuition eauto.
+    apply A. eapply perm_pop_stage in H0; eauto. apply H0. auto.
+Qed.
+
+Theorem record_frame_safe_extends:
+  forall m1 m1' m2 m2' fr,
+  extends m1 m2 ->
+  record_frame m1 fr = Some m1' ->
+  record_frame m2 fr = Some m2' ->
+  extends m1' m2'.
+Proof.
+  intros. inv H.
+  constructor.
+  - apply support_record_frame in H0.
+    apply support_record_frame in H1.
+    congruence.
+  - eapply record_frame_right_inj with (m1 := m1'); eauto.
+    eapply record_frame_left_inj; eauto.
+  - intros. exploit mext_perm_inv0.
+    eapply perm_record_frame in H1; eauto. apply H1 in H. apply H.
+    intros [A|A].
+    eapply perm_record_frame in H0; eauto. left. apply H0. auto.
+    right; intuition eauto.
+    apply A. eapply perm_record_frame in H0; eauto. apply H0. auto.
+Qed.
+
+Theorem record_frame_extends:
+  forall m1 m1' m2 fr,
+  extends m1 m2 ->
+  record_frame m1 fr= Some m1' ->
+  exists m2', record_frame m2 fr = Some m2' /\
+    extends m1' m2'.
+Proof.
+  intros. inv H.
+  apply record_frame_size1 in H0 as SIZE.
+  assert ({m2':mem|record_frame m2 fr = Some m2'}).
+  apply request_record_frame. auto.
+  apply record_frame_nonempty in H0. congruence. rewrite <- mext_sup0. lia.
+  destruct X as [m2' RECORD]. exists m2'. split. auto.
+  constructor.
+  - apply support_record_frame in H0.
+    apply support_record_frame in RECORD.
+    congruence.
+  - eapply record_frame_right_inj with (m1 := m1'); eauto.
+    eapply record_frame_left_inj; eauto.
+  - intros. exploit mext_perm_inv0.
+    eapply perm_record_frame in RECORD; eauto. apply RECORD in H. apply H.
+    intros [A|A].
+    eapply perm_record_frame in H0; eauto. left. apply H0. auto.
+    right; intuition eauto.
+    apply A. eapply perm_record_frame in H0; eauto. apply H0. auto.
+Qed.
+(*
+Theorem pop_stage_left_extends : forall m1 m1' m2,
+    extends m1 m2 ->
+    pop_stage m1 = Some m1' ->
+    extends m1' m2.
+Proof.
+  intros. inv H. constructor.
+  - erewrite <- supp_pop_stage; eauto.
+  - eapply pop_stage_left_inj; eauto.
+  - intros. apply mext_perm_inv0 in H. destruct H.
+    left. eapply perm_pop_stage in H0. apply H0. auto.
+    right. eapply perm_pop_stage in H0. intro. apply H.
+    apply H0. auto.
+Qed.
+
+Theorem pop_stage_right_extends' : forall m1 m2 m2',
+    extends' m1 m2 ->
+    pop_stage m2 = Some m2' ->
+    extends' m1 m2'.
+Proof.
+  intros. inv H. constructor.
+  - rewrite <- (supp_pop_stage _ _ H0). auto.
+  - eapply pop_stage_right_inj; eauto.
+  - intros. eapply mext_perm_inv0.
+    rewrite perm_pop_stage; eauto.
+Qed.
+
+Theorem push_stage_left_extends' : forall m1 m1' m2,
+    extends' m1 m2 ->
+    push_stage m1 = m1' ->
+    extends' m1' m2.
+Proof.
+  intros. inv H. constructor; eauto.
+  eapply push_stage_left_inj; eauto.
+Qed.
+
+Lemma push_stage_right_extends' : forall m1 m2,
+    Mem.extends' m1 m2 -> Mem.extends' m1 (Mem.push_stage m2).
+Proof.
+  intros. inv H. constructor; eauto.
+  eapply push_stage_right_inj; eauto.
+Qed.
+*)
 Theorem alloc_extends:
   forall m1 m2 lo1 hi1 b m1' lo2 hi2,
   extends m1 m2 ->
@@ -5290,6 +6004,33 @@ Proof.
   intuition eauto using perm_storebytes_1, perm_storebytes_2.
 Qed.
 
+Theorem push_stage_inject:
+  forall f m1 m2,
+    inject f m1 m2 ->
+    inject f (push_stage m1) (push_stage m2).
+Proof.
+  intros. inversion H. constructor; auto.
+  - inv mi_inj0. constructor; auto.
+Qed.
+
+Theorem push_stage_left_inject:
+  forall f m1 m2,
+    inject f m1 m2 ->
+    inject f (push_stage m1) m2.
+Proof.
+  intros. inv H. constructor; auto.
+  inv mi_inj0. constructor; auto.
+Qed.
+
+Theorem push_stage_right_inject:
+  forall f m1 m2,
+    inject f m1 m2 ->
+    inject f m1 (push_stage m2).
+Proof.
+  intros. inv H. constructor; auto.
+  inv mi_inj0. constructor; auto.
+Qed.
+
 (* Preservation of allocations *)
 
 Theorem alloc_right_inject:
@@ -5601,6 +6342,134 @@ Proof.
   intros [f' [A [B [C D]]]].
   exists f'; exists m2'; exists b2; auto.
 Qed.
+
+(* Preservation of [pop_stage] operations *)
+
+Lemma pop_stage_left_inject:
+  forall f m1 m2 m1',
+    inject f m1 m2 ->
+    pop_stage m1 = Some m1' ->
+    inject f m1' m2.
+Proof.
+  intros. inversion H. constructor; auto.
+  - eapply pop_stage_left_inj; eauto.
+  - eauto with mem.
+  - red; intros. eapply mi_no_overlap0; eauto.
+    rewrite perm_pop_stage. apply H4. auto.
+    rewrite perm_pop_stage. apply H5. auto.
+  - intros. eapply mi_representable0; eauto.
+    destruct H2. left.
+    rewrite perm_pop_stage; eauto. right.
+    rewrite perm_pop_stage; eauto.
+  - intros. exploit mi_perm_inv0; eauto. intros [H'|H'].
+    left. rewrite <- perm_pop_stage; eauto.
+    right. rewrite <- perm_pop_stage; eauto.
+Qed.
+
+Lemma pop_stage_right_inject:
+  forall f m1 m2 m2',
+    inject f m1 m2 ->
+    pop_stage m2 = Some m2' ->
+    inject f m1 m2'.
+Proof.
+  intros. inversion H. constructor; eauto.
+  eapply pop_stage_right_inj; eauto.
+  intros. eauto with mem.
+  intros. rewrite <- perm_pop_stage in H2; eauto.
+Qed.
+
+Theorem pop_stage_parallel_inject:
+  forall f m1 m2 m1',
+  inject f m1 m2 ->
+  pop_stage m1 = Some m1' ->
+  astack(support m2) <> nil ->
+  exists m2', pop_stage m2 = Some m2' /\
+  inject f m1' m2'.
+Proof.
+  intros. inversion H.
+  destruct (nonempty_pop_stage _ H1) as [m2' POP].
+  exists m2'. split. auto.
+  constructor; auto.
+  - eapply pop_stage_right_inj with (m1 := m1'); eauto.
+    eapply pop_stage_left_inj; eauto.
+  - eauto with mem.
+  - eauto with mem.
+  - red. intros.
+    rewrite <- perm_pop_stage in H5; eauto.
+    rewrite <- perm_pop_stage in H6; eauto.
+  - intros. eapply mi_representable0; eauto.
+    destruct H3. left. rewrite perm_pop_stage; eauto.
+    right. rewrite perm_pop_stage; eauto.
+  - intros. exploit mi_perm_inv0; eauto.
+    rewrite <- perm_pop_stage in H3; eauto. intros [A|A].
+    left. rewrite <- perm_pop_stage; eauto.
+    right. rewrite <- perm_pop_stage; eauto.
+Qed.
+
+Lemma record_frame_left_inject:
+  forall f m1 m2 m1' fr,
+    inject f m1 m2 ->
+    record_frame m1 fr = Some m1' ->
+    inject f m1' m2.
+Proof.
+  intros. inversion H. constructor; auto.
+  - eapply record_frame_left_inj; eauto.
+  - eauto with mem.
+  - red; intros. eapply mi_no_overlap0; eauto.
+    rewrite perm_record_frame; eauto.
+    rewrite perm_record_frame; eauto.
+  - intros. eapply mi_representable0; eauto.
+    destruct H2. left.
+    rewrite perm_record_frame; eauto. right.
+    rewrite perm_record_frame; eauto.
+  - intros. exploit mi_perm_inv0; eauto. intros [H'|H'].
+    left. rewrite <- perm_record_frame; eauto.
+    right. rewrite <- perm_record_frame; eauto.
+Qed.
+
+Lemma record_frame_right_inject:
+  forall f m1 m2 m2' fr,
+    inject f m1 m2 ->
+    record_frame m2 fr = Some m2' ->
+    inject f m1 m2'.
+Proof.
+  intros. inversion H. constructor; eauto.
+  eapply record_frame_right_inj; eauto.
+  intros. eauto with mem.
+  intros. rewrite <- perm_record_frame in H2; eauto.
+Qed.
+
+Theorem record_frame_parallel_inject:
+  forall f m1 m2 m1' fr ,
+  inject f m1 m2 ->
+  record_frame m1 fr = Some m1' ->
+  astack(support m2) <> nil ->
+  stack_size (astack(support m2)) <= stack_size(astack(support m1)) ->
+  exists m2', record_frame m2 fr = Some m2' /\
+  inject f m1' m2'.
+Proof.
+  intros. inversion H.
+  eapply request_record_frame in H1; eauto.
+  destruct H1 as [m2' RECORD].
+  exists m2'. split. eauto.
+  constructor; auto.
+  - eapply record_frame_right_inj with (m1 := m1'); eauto.
+    eapply record_frame_left_inj; eauto.
+  - eauto with mem.
+  - eauto with mem.
+  - red. intros.
+    rewrite <- perm_record_frame in H5; eauto.
+    rewrite <- perm_record_frame in H6; eauto.
+  - intros. eapply mi_representable0; eauto.
+    destruct H3. left. rewrite perm_record_frame; eauto.
+    right. rewrite perm_record_frame; eauto.
+  - intros. exploit mi_perm_inv0; eauto.
+    rewrite <- perm_record_frame in H3; eauto. intros [A|A].
+    left. rewrite <- perm_record_frame; eauto.
+    right. rewrite <- perm_record_frame; eauto.
+  - apply record_frame_size1 in H0. lia.
+Qed.
+
 
 (** Preservation of [free] operations *)
 
@@ -6040,6 +6909,341 @@ Proof.
   repeat rewrite Z.add_0_r. intros [m'' [A B]]. congruence.
 Qed.
 
+Section MEMIFF.
+
+Record iff (m1 m2: mem) : Prop := mk_iff {
+  global_iff:
+    Mem.global (Mem.support m1) = Mem.global (Mem.support m2);
+  stack_iff:
+    Mem.stack (Mem.support m1) = Mem.stack (Mem.support m2);
+  access_iff:
+    m1.(Mem.mem_access) = m2.(Mem.mem_access);
+  contents_iff:
+    m1.(Mem.mem_contents) = m2.(Mem.mem_contents)
+}.
+
+Lemma iff_refl:
+  forall m, iff m m.
+Proof.
+  intros. constructor; auto. Qed.
+
+Lemma iff_comm:
+  forall m1 m2, iff m1 m2 -> iff m2 m1.
+Proof.
+  intros. inv H. constructor; auto.
+Qed.
+
+Lemma iff_trans:
+  forall m1 m2 m3, iff m1 m2 -> iff m2 m3 -> iff m1 m3.
+Proof.
+  intros. inv H. inv H0.
+  constructor; congruence.
+Qed.
+
+Lemma valid_block_iff:
+  forall m m' b,
+  iff m m' -> valid_block m b -> valid_block m' b.
+Proof.
+  unfold valid_block; intros. destruct b; simpl in *.
+  erewrite <- stack_iff; eauto. erewrite <- global_iff; eauto.
+Qed.
+
+Lemma perm_iff:
+  forall m m' b ofs k p,
+  iff m m' ->
+  perm m b ofs k p <-> perm m' b ofs k p.
+Proof.
+  intros. destruct H. unfold perm. rewrite access_iff0.
+  reflexivity.
+Qed.
+
+
+Lemma range_perm_iff:
+  forall m m' b lo hi k p,
+    iff m m' ->
+    range_perm m b lo hi k p = range_perm m' b lo hi k p.
+Proof.
+  unfold range_perm. intros.
+  inv H.
+  unfold perm. rewrite access_iff0.
+  auto.
+Qed.
+
+Lemma valid_access_iff:
+  forall m1 m2 chunk b ofs p,
+    iff m1 m2 ->
+    valid_access m1 chunk b ofs p <-> valid_access m2 chunk b ofs p.
+Proof.
+  intros. inv H.
+  unfold valid_access.
+  unfold range_perm.
+  unfold perm.
+  rewrite access_iff0. reflexivity.
+Qed.
+
+Lemma load_iff:
+  forall m1 m2 chunk b ofs,
+    iff m1 m2 ->
+    load chunk m1 b ofs = load chunk m2 b ofs.
+Proof.
+  intros. inversion H. unfold load.
+  destruct (valid_access_dec m1 chunk b ofs Readable).
+  - rewrite pred_dec_true. rewrite contents_iff0. reflexivity.
+    rewrite <- valid_access_iff; eauto.
+  - rewrite pred_dec_false. auto.
+    rewrite <- valid_access_iff; eauto.
+Qed.
+
+Lemma loadv_iff:
+  forall m1 m2 chunk  addr,
+    iff m1 m2 ->
+    loadv chunk m1 addr = loadv chunk m2 addr.
+Proof.
+  intros. inversion H. unfold loadv.
+  destruct addr; eauto.
+  apply load_iff. eauto.
+Qed.
+
+Lemma loadbytes_iff:
+  forall m1 m2 b ofs n,
+    iff m1 m2 ->
+    loadbytes m1 b ofs n = loadbytes m2 b ofs n.
+Proof.
+  intros. inversion H.
+  unfold loadbytes.
+  repeat destr.
+  erewrite range_perm_iff in r; eauto. congruence.
+  erewrite <- range_perm_iff in r; eauto. congruence.
+Qed.
+
+Lemma store_iff:
+  forall m1 m2 m1' chunk b ofs v,
+    iff m1 m2 ->
+    store chunk m1 b ofs v = Some m1' ->
+    exists m2',
+      store chunk m2 b ofs v = Some m2'
+      /\ iff m1' m2'.
+Proof.
+  intros m1 m2 m1' chunk b ofs v IFF STORE.
+  inversion IFF.
+  apply store_valid_access_3 in STORE as VALID.
+  apply store_valid_access_3 in STORE as VALID'.
+  erewrite valid_access_iff in VALID'; eauto.
+  eapply valid_access_store in VALID' as X.
+  destruct X as [m2' STORE'].
+  exists m2'. split. eauto.
+  unfold store in *.
+  rewrite pred_dec_true in STORE; eauto.
+  rewrite pred_dec_true in STORE'; eauto.
+  inv STORE. inv STORE'.
+  constructor; auto. simpl.
+  rewrite contents_iff0. auto.
+Qed.
+
+Lemma storev_iff:
+  forall m1 m2 m1' chunk addr v,
+    iff m1 m2 ->
+    storev chunk m1 addr v = Some m1' ->
+    exists m2',
+      storev chunk m2 addr v = Some m2'
+      /\ iff m1' m2'.
+Proof.
+  intros m1 m2 m1' chunk addr v IFF.
+  unfold storev. destruct addr; try congruence; eauto.
+  apply store_iff. auto.
+Qed.
+
+Lemma storebytes_iff:
+  forall m1 m2 m1' b ofs bytes,
+    iff m1 m2 ->
+    storebytes m1 b ofs bytes = Some m1' ->
+    exists m2',
+      storebytes m2 b ofs bytes = Some m2'
+      /\ iff m1' m2'.
+Proof.
+  intros. inversion H.
+  apply storebytes_range_perm in H0 as PERM.
+  apply storebytes_range_perm in H0 as PERM'.
+  erewrite range_perm_iff in PERM'; eauto.
+  apply range_perm_storebytes in PERM' as X.
+  destruct X as [m2' STORE'].
+  exists m2'. split. auto. unfold storebytes in *.
+  destr_in H0. inv H0.
+  destr_in STORE'. inv STORE'.
+  constructor; auto. simpl.
+  rewrite contents_iff0. auto.
+Qed.
+
+Lemma push_stage_iff:
+  forall m, iff m (Mem.push_stage m).
+Proof.
+  intros. constructor; auto.
+Qed.
+
+Lemma pop_stage_iff:
+  forall m m', Mem.pop_stage m = Some m' -> iff m m'.
+Proof.
+  intros. unfold pop_stage in H.
+  destruct (astack (support m)). discriminate.
+  inv H.
+  constructor; auto.
+Qed.
+
+Lemma record_frame_iff:
+  forall m m' fr, Mem.record_frame m fr = Some m' -> iff m m'.
+Proof.
+  intros. unfold record_frame in H.
+  destr_in H. destr_in H. inv H.
+  constructor; auto.
+Qed.
+
+Lemma push_stage_right_iff:
+  forall m1 m2,
+    iff m1 m2 -> iff m1 (Mem.push_stage m2).
+Proof.
+  intros.
+  eapply iff_trans.  eauto.  eapply push_stage_iff.
+Qed.
+
+Lemma push_stage_left_iff:
+  forall m1 m2,
+    iff m1 m2 -> iff (Mem.push_stage m1) m2.
+Proof.
+  intros.
+  eapply iff_trans. eapply iff_comm. eapply push_stage_iff; eauto. eauto.
+Qed.
+
+Lemma pop_stage_right_iff:
+  forall m1 m2 m2',
+    iff m1 m2 -> Mem.pop_stage m2 = Some m2' -> iff m1 m2'.
+Proof.
+  intros.
+  eapply iff_trans. eauto. eapply pop_stage_iff. eauto.
+Qed.
+
+Lemma pop_stage_left_iff:
+  forall m1 m2 m1',
+    iff m1 m2 -> Mem.pop_stage m1 = Some m1' -> iff m1' m2.
+Proof.
+  intros.
+  eapply iff_trans. eapply iff_comm. eapply pop_stage_iff; eauto. eauto.
+Qed.
+
+Lemma free_parallel_iff:
+  forall m1 m2 m1' b lo hi,
+    iff m1 m2 ->
+    free m1 b lo hi = Some m1' ->
+    exists m2', free m2 b lo hi = Some m2'
+           /\ iff m1' m2'.
+Proof.
+  intros.
+  apply free_range_perm in H0 as PERM.
+  apply free_range_perm in H0 as PERM'.
+  erewrite range_perm_iff in PERM'; eauto.
+  eapply range_perm_free in PERM' as X.
+  destruct X as [m2' FREE].
+  exists m2'. split. auto.
+  unfold free in *.
+  rewrite pred_dec_true in *; eauto.
+  inv H0. inv FREE. unfold unchecked_free.
+  inv H. constructor; eauto. simpl.
+  rewrite access_iff0. eauto.
+Qed.
+
+Lemma alloc_frame_iff :
+  forall m1 m2 m1' id path,
+    iff m1 m2 ->
+    alloc_frame m1 id = (m1',path) ->
+    exists m2', alloc_frame m2 id = (m2',path) /\ iff m1' m2'.
+Proof.
+  intros. inversion H. caseEq (alloc_frame m2 id). intros.
+  exists m. split. apply path_alloc_frame in H0.
+  apply path_alloc_frame in H1. unfold sup_npath in *. congruence.
+  inv H0. inv H1.
+  constructor; simpl; auto; unfold sup_incr_frame; rewrite stack_iff0; destr.
+Qed.
+
+Lemma return_frame_iff :
+  forall m1 m2 m1',
+  iff m1 m2 ->
+  return_frame m1 = Some m1' ->
+  exists m2', return_frame m2 = Some m2' /\ iff m1' m2'.
+Proof.
+  intros. inversion H.
+  apply return_frame_active in H0 as H1. rewrite stack_iff0 in H1.
+  apply active_return_frame in H1 as H2. destruct H2 as [m2' H3].
+  exists m2'. split. eauto. unfold return_frame in *. destr_in H0.
+  destr_in H3. inv H0. inv H3.
+  constructor; simpl; auto.
+  unfold sup_return_frame'.
+  unfold sup_return_frame.
+  rewrite stack_iff0. destruct (return_stree (stack (support m2))) eqn:?. destruct p. simpl. auto. auto.
+unfold sup_return_frame'.
+  unfold sup_return_frame.
+  rewrite stack_iff0. destruct (return_stree (stack (support m2))) eqn:?. destruct p. simpl. auto. auto.
+Qed.
+
+Lemma alloc_parallel_iff:
+  forall m1 m2 m1' lo hi b,
+    iff m1 m2 ->
+    alloc m1 lo hi = (m1',b) ->
+    exists m2', alloc m2 lo hi = (m2',b)
+           /\ iff m1' m2'.
+Proof.
+  intros.  inversion H.
+  caseEq (alloc m2 lo hi).
+  intros.
+  assert (b = b0).
+   apply alloc_result in H0.
+   apply alloc_result in H1.
+  unfold nextblock in *. unfold fresh_block in *.
+  rewrite stack_iff0 in H0. congruence.
+  subst.
+  exists m. split. auto.
+  unfold alloc in *. inv H0. inv H1.
+  constructor; simpl; try congruence; unfold sup_incr;
+  rewrite stack_iff0; destr.
+Qed.
+
+Lemma pop_stage_safe_iff:
+  forall m1 m2 m1' m2',
+    iff m1 m2 ->
+    pop_stage m1 = Some m1' ->
+    pop_stage m2 = Some m2' ->
+    iff m1' m2'.
+Proof.
+  intros.
+  eapply iff_trans. eapply iff_comm.
+  eapply pop_stage_iff; eauto.
+  eapply iff_trans. eauto.
+  eapply pop_stage_iff; eauto.
+Qed.
+
+Lemma push_stage_safe_iff:
+  forall m1 m2,
+    iff m1 m2 -> iff (push_stage m1) (push_stage m2).
+Proof.
+  intros. inv H. constructor; auto.
+Qed.
+
+
+Lemma record_frame_safe_iff:
+  forall m1 m2 m1' m2' fr,
+    iff m1 m2 ->
+    record_frame m1 fr = Some m1' ->
+    record_frame m2 fr = Some m2' ->
+    iff m1' m2'.
+Proof.
+  intros.
+  eapply iff_trans. eapply iff_comm.
+  eapply record_frame_iff; eauto.
+  eapply iff_trans. eauto.
+  eapply record_frame_iff; eauto.
+Qed.
+
+End MEMIFF.
+
+
 (** * Invariance properties between two memory states *)
 
 Section UNCHANGED_ON.
@@ -6259,6 +7463,7 @@ Proof.
 Qed.
 
 End Mem.
+
 Notation mem := Mem.mem.
 Notation sup := Mem.sup.
 Notation sup_In := Mem.sup_In.
@@ -6329,3 +7534,4 @@ Hint Resolve
   Mem.valid_access_free_inv_2
   Mem.unchanged_on_refl
 : mem.
+
