x86/Op.v
@@ -1427,6 +1427,72 @@ Qed.
 
 End EVAL_LESSDEF.
 
+Section EVAL_IFF.
+
+Variable F V: Type.
+Variable genv: Genv.t F V.
+
+Lemma valid_pointer_memiff : forall m1 m2 b ofs,
+    Mem.iff m1 m2 -> Mem.valid_pointer m1 b ofs = true <-> Mem.valid_pointer m2 b ofs = true.
+Proof. intros. inv H.
+       transitivity (Mem.perm m1 b ofs Cur Nonempty).
+       apply Mem.valid_pointer_nonempty_perm.
+       transitivity (Mem.perm m2 b ofs Cur Nonempty).
+       unfold Mem.perm. rewrite access_iff. reflexivity.
+       symmetry. apply Mem.valid_pointer_nonempty_perm.
+Qed.
+
+Lemma valid_pointer_memiff1 : forall m1 m2 b ofs,
+    Mem.iff m1 m2 -> Mem.valid_pointer m1 b ofs = Mem.valid_pointer m2 b ofs.
+Proof. intros.
+       destruct (Mem.valid_pointer m1 b ofs) eqn:vp1.
+       generalize (valid_pointer_memiff b ofs H). intros.
+       apply H0 in vp1. rewrite vp1. auto.
+       destruct (Mem.valid_pointer m2 b ofs) eqn:vp2.
+       eapply valid_pointer_memiff in vp2; eauto. auto.
+Qed.
+
+Lemma eval_condition_memiff:
+    forall  (m m0 : mem) (cond : condition) (vl : list val),
+      Mem.iff m m0 ->
+      eval_condition cond vl m =
+      eval_condition cond vl m0.
+Proof.
+    intros m m0 cond vl H6.
+    unfold eval_condition. destruct cond; auto.
+    unfold Val.cmplu_bool.
+    unfold Val.cmpu_bool.
+    repeat destr.
+    repeat (erewrite (valid_pointer_memiff1 _ _ H6) in Heqb1). congruence.
+    repeat (erewrite (valid_pointer_memiff1 _ _ H6) in Heqb1). congruence.
+    repeat (erewrite (valid_pointer_memiff1 _ _ H6) in Heqb1). congruence.
+    repeat (erewrite (valid_pointer_memiff1 _ _ H6) in Heqb1). congruence.
+    repeat (erewrite (valid_pointer_memiff1 _ _ H6) in Heqb0). congruence.
+    repeat (erewrite (valid_pointer_memiff1 _ _ H6) in Heqb0). congruence.
+    repeat (erewrite (valid_pointer_memiff1 _ _ H6) in Heqb0). congruence.
+    repeat (erewrite (valid_pointer_memiff1 _ _ H6) in Heqb0). congruence.
+    unfold Val.cmplu_bool.
+    unfold Val.cmpu_bool.
+    repeat destr.
+    repeat (erewrite (valid_pointer_memiff1 _ _ H6) in Heqb1). congruence.
+    repeat (erewrite (valid_pointer_memiff1 _ _ H6) in Heqb1). congruence.
+Qed.
+
+Lemma eval_operation_memiff:
+  forall sp op vl v m1 m2,
+    Mem.iff m1 m2 ->
+    eval_operation genv sp op vl m1 = Some v ->
+    eval_operation genv sp op vl m2 = Some v.
+Proof.
+  intros.
+  unfold eval_operation in *. destruct op; auto.
+  erewrite eval_condition_memiff in H0; eauto.
+  repeat destr.
+  erewrite eval_condition_memiff in H0; eauto.
+Qed.
+End EVAL_IFF.
+
+
 (** Compatibility of the evaluation functions with memory injections. *)
 
 Section EVAL_INJECT.
