Makefile
@@ -91,6 +91,7 @@ BACKEND=\
   SelectLongproof.v Selectionproof.v \
   Registers.v RTL.v \
   RTLgen.v RTLgenspec.v RTLgenproof.v \
+  RTLmach.v RTLmachproof.v \
   Renumber.v Renumberproof.v \
   RTLtyping.v \
   Kildall.v Liveness.v \
